LeanHoG/Invariant.lean
@@ -1,5 +1,6 @@
 import LeanHoG.Invariant.Bipartite
 import LeanHoG.Invariant.ConnectedComponents
 import LeanHoG.Invariant.G6
+import LeanHoG.Invariant.HamiltonianCycle
 import LeanHoG.Invariant.HamiltonianPath
 import LeanHoG.Invariant.NeighborhoodMap
